theories/zoo_saturn/queue_mpsc_3__code.v
@@ -5,28 +5,28 @@ Require Import zoo_std.clist.
 Require Import zoo_std.domain.
 Require Import zoo.options.
 
-Notation "'mpsc_queue_3٠front'" := (
-  in_type "zoo_saturn.mpsc_queue_3.t" 0
+Notation "'queue_mpsc_3٠front'" := (
+  in_type "zoo_saturn.queue_mpsc_3.t" 0
 )(in custom zoo_field
 ).
-Notation "'mpsc_queue_3٠back'" := (
-  in_type "zoo_saturn.mpsc_queue_3.t" 1
+Notation "'queue_mpsc_3٠back'" := (
+  in_type "zoo_saturn.queue_mpsc_3.t" 1
 )(in custom zoo_field
 ).
 
-Definition mpsc_queue_3٠create : val :=
+Definition queue_mpsc_3٠create : val :=
   𝗳𝘂𝗻 ⎽ ->
     { §clist٠Open, §clist٠Open }.
 
-Definition mpsc_queue_3٠is_empty : val :=
+Definition queue_mpsc_3٠is_empty : val :=
   𝗳𝘂𝗻 "t" ->
-    𝗺𝗮𝘁𝗰𝗵 "t".{mpsc_queue_3٠front} 𝘄𝗶𝘁𝗵
+    𝗺𝗮𝘁𝗰𝗵 "t".{queue_mpsc_3٠front} 𝘄𝗶𝘁𝗵
     | clist٠Closed ->
         true
     | clist٠Cons ⎽ ⎽ ->
         false
     | clist٠Open ->
-        𝗺𝗮𝘁𝗰𝗵 "t".{mpsc_queue_3٠back} 𝘄𝗶𝘁𝗵
+        𝗺𝗮𝘁𝗰𝗵 "t".{queue_mpsc_3٠back} 𝘄𝗶𝘁𝗵
         | clist٠Cons ⎽ ⎽ ->
             false
         | ⎽ ->
@@ -34,25 +34,25 @@ Definition mpsc_queue_3٠is_empty : val :=
         𝗲𝗻𝗱
     𝗲𝗻𝗱.
 
-Definition mpsc_queue_3٠push_front : val :=
+Definition queue_mpsc_3٠push_front : val :=
   𝗳𝘂𝗻 "t" "v" ->
-    𝗺𝗮𝘁𝗰𝗵 "t".{mpsc_queue_3٠front} 𝘄𝗶𝘁𝗵
+    𝗺𝗮𝘁𝗰𝗵 "t".{queue_mpsc_3٠front} 𝘄𝗶𝘁𝗵
     | clist٠Closed ->
         true
     | ⎽ 𝗮𝘀 "front" ->
-        "t" <-{mpsc_queue_3٠front} ‘clist٠Cons[ "v", "front" ] ⍮
+        "t" <-{queue_mpsc_3٠front} ‘clist٠Cons[ "v", "front" ] ⍮
         false
     𝗲𝗻𝗱.
 
-Definition mpsc_queue_3٠push_back : val :=
+Definition queue_mpsc_3٠push_back : val :=
   𝗿𝗲𝗰 "push_back" "t" "v" ->
-    𝗺𝗮𝘁𝗰𝗵 "t".{mpsc_queue_3٠back} 𝘄𝗶𝘁𝗵
+    𝗺𝗮𝘁𝗰𝗵 "t".{queue_mpsc_3٠back} 𝘄𝗶𝘁𝗵
     | clist٠Closed ->
         true
     | ⎽ 𝗮𝘀 "back" ->
         𝗶𝗳
           𝗰𝗮𝘀
-            "t".[mpsc_queue_3٠back]
+            "t".[queue_mpsc_3٠back]
             "back"
             ‘clist٠Cons[ "v", "back" ]
         𝘁𝗵𝗲𝗻 (
@@ -63,17 +63,17 @@ Definition mpsc_queue_3٠push_back : val :=
         )
     𝗲𝗻𝗱.
 
-Definition mpsc_queue_3٠pop : val :=
+Definition queue_mpsc_3٠pop : val :=
   𝗳𝘂𝗻 "t" ->
-    𝗺𝗮𝘁𝗰𝗵 "t".{mpsc_queue_3٠front} 𝘄𝗶𝘁𝗵
+    𝗺𝗮𝘁𝗰𝗵 "t".{queue_mpsc_3٠front} 𝘄𝗶𝘁𝗵
     | clist٠Closed ->
         §None
     | clist٠Cons "v" "front" ->
-        "t" <-{mpsc_queue_3٠front} "front" ⍮
+        "t" <-{queue_mpsc_3٠front} "front" ⍮
         ‘Some( "v" )
     | clist٠Open ->
         𝗺𝗮𝘁𝗰𝗵
-          𝘅𝗰𝗵𝗴 "t".[mpsc_queue_3٠back] §clist٠Open
+          𝘅𝗰𝗵𝗴 "t".[queue_mpsc_3٠back] §clist٠Open
         𝘄𝗶𝘁𝗵
         | clist٠Open ->
             §None
@@ -82,7 +82,7 @@ Definition mpsc_queue_3٠pop : val :=
               clist٠rev_app "back" §clist٠Open
             𝘄𝗶𝘁𝗵
             | clist٠Cons "v" "front" ->
-                "t" <-{mpsc_queue_3٠front} "front" ⍮
+                "t" <-{queue_mpsc_3٠front} "front" ⍮
                 ‘Some( "v" )
             | ⎽ ->
                 𝗳𝗮𝗶𝗹
@@ -90,17 +90,17 @@ Definition mpsc_queue_3٠pop : val :=
         𝗲𝗻𝗱
     𝗲𝗻𝗱.
 
-Definition mpsc_queue_3٠close : val :=
+Definition queue_mpsc_3٠close : val :=
   𝗳𝘂𝗻 "t" ->
     𝗺𝗮𝘁𝗰𝗵
-      𝘅𝗰𝗵𝗴 "t".[mpsc_queue_3٠back] §clist٠Closed
+      𝘅𝗰𝗵𝗴 "t".[queue_mpsc_3٠back] §clist٠Closed
     𝘄𝗶𝘁𝗵
     | clist٠Closed ->
         true
     | ⎽ 𝗮𝘀 "back" ->
-        "t" <-{mpsc_queue_3٠front}
+        "t" <-{queue_mpsc_3٠front}
           clist٠app
-            "t".{mpsc_queue_3٠front}
+            "t".{queue_mpsc_3٠front}
             (clist٠rev_app "back" §clist٠Closed) ⍮
         false
     𝗲𝗻𝗱.
