theories/zoo_saturn/queue_mpsc_3__opaque.v
@@ -1,0 +1,8 @@
+Require Import zoo_saturn.queue_mpsc_3__code.
+
+#[global] Opaque queue_mpsc_3٠create.
+#[global] Opaque queue_mpsc_3٠is_empty.
+#[global] Opaque queue_mpsc_3٠push_front.
+#[global] Opaque queue_mpsc_3٠push_back.
+#[global] Opaque queue_mpsc_3٠pop.
+#[global] Opaque queue_mpsc_3٠close.
